proof/NormalTypeSystemSimp.v
@@ -14,78 +14,134 @@ Import CoreLangSimp.
 
 Definition context := partial_map ty.
 
-Reserved Notation "Gamma '|-' t '\in' T" (at level 40).
+Reserved Notation "Gamma '|-' t '\Tin' T" (at level 40).
 
 Inductive has_type : context -> tm -> ty -> Prop :=
 | T_Exn : forall Gamma T, has_type Gamma texn T
-| T_Value : forall Gamma value T,
-    value_has_type Gamma value T -> has_type Gamma (tvalue value) T
+| T_Value : forall Gamma value T, value_has_type Gamma value T -> has_type Gamma (tvalue value) T
 | T_Lete : forall Gamma x e1 e2 T1 T2,
     has_type Gamma e1 T1 ->
     has_type (update Gamma x T1) e2 T2 ->
     has_type Gamma (tlete x e1 e2) T2
-| T_LetOp : forall Gamma x op v1 v2 e2 T2,
-    value_has_type Gamma v1 (TBasic TNat) ->
-    value_has_type Gamma v2 (TBasic TNat) ->
-    has_type (update Gamma x (TBasic (op_ret_ty op))) e2 T2 ->
-    has_type Gamma (tletbiop x op v1 v2 e2) T2
+| T_LetOp : forall Gamma x op v1 v2 e (T1 T2 Tx: base_ty) T,
+    value_has_type Gamma v1 T1 ->
+    value_has_type Gamma v2 T2 ->
+    ty_of_op op = T1 t--> (T2 t--> Tx) ->
+    has_type (update Gamma x Tx) e T ->
+    has_type Gamma (tletbiop x op v1 v2 e) T
 | T_LetApp : forall Gamma y v_x v_f e2 T_x T_y T2,
     value_has_type Gamma v_x T_x ->
     value_has_type Gamma v_f (TArrow T_x T_y) ->
     has_type (update Gamma y T_y) e2 T2 ->
     has_type Gamma (tletapp y v_f v_x e2) T2
+| T_Matchb: forall Gamma v e1 e2 T,
+    value_has_type Gamma v TBool ->
+    has_type Gamma e1 T ->
+    has_type Gamma e2 T ->
+    has_type Gamma (tmatchb v e1 e2) T
 with value_has_type : context -> value -> ty -> Prop :=
-| T_ConstantB : forall Gamma b, value_has_type Gamma (vconst (cbool b)) (TBasic TBool)
-| T_ConstantI : forall Gamma n, value_has_type Gamma (vconst (cnat n)) (TBasic TNat)
+| T_Const : forall Gamma (c: constant), value_has_type Gamma c (ty_of_const c)
+| T_Op : forall Gamma (op: biop), value_has_type Gamma (vbiop op) (ty_of_op op)
 | T_Var : forall Gamma x T, Gamma x = Some T -> value_has_type Gamma (vvar x) T
 | T_Lam : forall Gamma x T11 T12 t12,
     has_type (update Gamma x T11) t12 T12 ->
     value_has_type Gamma (vlam x T11 t12) (TArrow T11 T12)
 
-where "Gamma '|-' t '\in' T" := (has_type Gamma t T).
+where "Gamma '|-' t '\Tin' T" := (has_type Gamma t T).
 Notation "Gamma '|-' t '\Vin' T" := (value_has_type Gamma t T) (at level 40).
 
 Global Hint Constructors has_type: core.
 Global Hint Constructors value_has_type: core.
 
-Lemma op_type_safe: forall op n1 n2, empty |- vconst (apply_op op n1 n2) \Vin TBasic (op_ret_ty op).
+Lemma eval_op_is_type_safe: forall Gamma op (c1 c2 c3: constant) (T1 T2 T3: base_ty),
+    Gamma |- c1 \Vin T1 -> Gamma |- c2 \Vin T2 ->
+                                 eval_op op c1 c2 c3 -> ty_of_op op = T1 t--> (T2 t--> T3) ->
+                                 empty |- c3 \Vin T3.
 Proof.
-  intro op.
-  destruct op; simpl; intros; auto.
+  intros Gamma op c1 c2 c3 T1 T2 T3 Hc1 Hc2 Heval Hop.
+  destruct Heval; inversion Hc1; subst; inversion Hc2; subst; inversion Hop; subst; constructor.
 Qed.
 
-Global Hint Resolve op_type_safe: core.
+Global Hint Resolve eval_op_is_type_safe: core.
 
-Lemma nat_value_n_exists: forall v, empty |- v \Vin (TBasic TNat) -> (exists n, v = (vconst (cnat n))).
-Proof.
-  intros.
-  destruct v; inversion H; subst; eauto.
-  - inversion H2.
-Qed.
-
-Lemma bool_value_b_exists: forall v, empty |- v \Vin (TBasic TBool) -> (exists b, v = (vconst (cbool b))).
+Lemma base_value_const_exists:
+  forall T v, empty |- v \Vin (TBase T) -> (exists c, v = vconst c).
 Proof.
   intros.
   destruct v; inversion H; subst; eauto.
   - inversion H2.
 Qed.
 
-Lemma basic_value_const_exists:
-  forall T v, empty |- v \Vin (TBasic T) -> (exists c, v = vconst c).
-Proof.
-  intros.
-  destruct v; inversion H; subst; eauto. inversion H2.
+Global Hint Resolve base_value_const_exists: core.
+
+Lemma nat_const_n_exists: forall Gamma (c: constant), Gamma |- c \Vin (TBase TNat) -> (exists (n: nat), c = n).
+Proof with eauto.
+  intros. destruct c; inversion H; subst...
 Qed.
 
-Lemma arrow_value_lam_exists: forall v T1 T2,
-    empty |- v \Vin (TArrow T1 T2) -> exists x e, v = vlam x T1 e.
-Proof.
-  intros.
-  destruct v; inversion H; subst; eauto.
-  - inversion H2.
+Global Hint Resolve nat_const_n_exists: core.
+
+Lemma bool_const_b_exists: forall Gamma (c: constant), Gamma |- c \Vin (TBase TBool) -> (exists (n: bool), c = n).
+Proof with eauto.
+  intros. destruct c; inversion H; subst...
 Qed.
 
-Lemma has_type_inv_value: forall Gamma v T, Gamma |- tvalue v \in T -> Gamma |- v \Vin T.
+Global Hint Resolve bool_const_b_exists: core.
+
+Lemma nat_value_n_exists: forall v, empty |- v \Vin (TBase TNat) -> (exists n, v = (vconst (cnat n))).
+Proof with eauto.
+  intros. assert (exists c, v = vconst c) as HH...
+  destruct HH as (c & Hc); subst... eapply nat_const_n_exists in H... destruct H; subst...
+Qed.
+
+Global Hint Resolve nat_value_n_exists: core.
+
+Lemma bool_value_b_exists: forall v, empty |- v \Vin (TBase TBool) -> (exists b, v = (vconst (cbool b))).
+Proof with eauto.
+  intros. assert (exists c, v = vconst c) as HH...
+  destruct HH as (c & Hc); subst... eapply bool_const_b_exists in H... destruct H; subst...
+Qed.
+
+Global Hint Resolve bool_value_b_exists: core.
+
+Lemma base_value_cid_exists:
+  forall Gamma T v, Gamma |- v \Vin (TBase T) -> ((exists c, v = vconst c) \/ (exists (name: string), v = name)).
+Proof.
+  intros.
+  destruct v.
+  - inversion H.
+  - inversion H; subst. left; eauto. right; eauto.
+  - inversion H.
+Qed.
+
+Global Hint Resolve base_value_cid_exists: core.
+
+Lemma nat_value_cid_exists: forall Gamma v, Gamma |- v \Vin (TBase TNat) ->
+                                               ((exists n, v = (vconst (cnat n))) \/ (exists (name: string), v = name)).
+Proof with eauto.
+  intros. assert ((exists c : constant, v = c) \/ (exists name : string, v = name)) as HH... destruct HH.
+  - left. destruct H0; subst... apply nat_const_n_exists in H... destruct H. exists x0. inversion H...
+  - right. destruct H0; subst...
+Qed.
+
+Lemma bool_value_cid_exists: forall Gamma v, Gamma |- v \Vin (TBase TBool) ->
+                                               ((exists n, v = (vconst (cbool n))) \/ (exists (name: string), v = name)).
+Proof with eauto.
+  intros. assert ((exists c : constant, v = c) \/ (exists name : string, v = name)) as HH... destruct HH.
+  - left. destruct H0; subst... apply bool_const_b_exists in H... destruct H. exists x0. inversion H...
+  - right. destruct H0; subst...
+Qed.
+
+(* Lemma arrow_value_lam_exists: forall v T1 T2, *)
+(*     empty |- v \Vin (TArrow T1 T2) -> exists x e, v = vlam x T1 e. *)
+(* Proof. *)
+(*   intros. *)
+(*   destruct v; inversion H; subst; eauto. *)
+(*   - destruct b; inversion H3; inversion H2. *)
+(*   - inversion H2. *)
+(* Qed. *)
+
+Lemma has_type_inv_value: forall Gamma v T, Gamma |- tvalue v \Tin T -> Gamma |- v \Vin T.
 Proof.
   intros.
   inversion H; subst; auto.
@@ -100,12 +156,13 @@ Qed.
 
 Lemma weakening : forall e T Gamma Gamma',
     includedin Gamma Gamma' ->
-    (Gamma  |- e \in T -> Gamma' |- e \in T).
+    (Gamma  |- e \Tin T -> Gamma' |- e \Tin T).
 Proof.
   intro e.
   apply (tm_mutual_rec
          (fun v => forall T Gamma Gamma', includedin Gamma Gamma' -> (Gamma  |- v \Vin T -> Gamma' |- v \Vin T))
-         (fun e => forall T Gamma Gamma', includedin Gamma Gamma' -> (Gamma  |- e \in T -> Gamma' |- e \in T))).
+         (fun e => forall T Gamma Gamma', includedin Gamma Gamma' -> (Gamma  |- e \Tin T -> Gamma' |- e \Tin T))).
+  - intros; inversion H0; subst; eauto 7 using includedin_update.
   - intros; inversion H0; subst; eauto 7 using includedin_update.
   - intros; inversion H1; subst; eauto 7 using includedin_update.
   - intros; inversion H0; subst; eauto 7 using includedin_update.
@@ -113,6 +170,7 @@ Proof.
   - intros; inversion H2; subst; eauto 7 using includedin_update.
   - intros; inversion H3; subst; eauto 7 using includedin_update.
   (* - intros. inversion H2; subst; eauto 7 using includedin_update. *)
+  - intros; inversion H3; subst; eauto 7 using includedin_update.
   - intros; inversion H3; subst; eauto 7 using includedin_update.
 Qed.
 
@@ -126,7 +184,7 @@ Proof.
 Qed.
 
 Lemma weakening_empty : forall Gamma t T,
-    empty |- t \in T  -> Gamma |- t \in T.
+    empty |- t \Tin T  -> Gamma |- t \Tin T.
 Proof.
   intros Gamma t T.
   eapply weakening.
@@ -137,15 +195,8 @@ Lemma value_weakening_empty : forall Gamma t T,
     empty |- t \Vin T  -> Gamma |- t \Vin T.
 Proof.
   intros Gamma t T H.
-  assert (empty |- (tvalue t) \in T). auto.
+  assert (empty |- (tvalue t) \Tin T). auto.
   apply weakening_empty with (Gamma:=Gamma) in H0. inversion H0; subst; auto.
-Qed.
-
-Lemma substitution_preserves_typing1:
-  (forall (c : constant) (Gamma : partial_map ty) (x : string) (U : ty) (v : value) (T : ty),
-      (x |-> U; Gamma) |- vconst c \Vin T -> empty |- v \Vin U -> Gamma |- [x := v ]v vconst c \Vin T).
-Proof.
-  intro c. induction c; intros; inversion H; clear H; subst; simpl; eauto.
 Qed.
 
 Lemma substitution_preserves_typing2:
@@ -163,25 +214,15 @@ Proof.
     apply T_Var. rewrite update_neq in H3; auto.
 Qed.
 
-Lemma substitution_preserves_typing5:
-  (forall v : value,
-      (forall (Gamma : partial_map ty) (x : string) (U : ty) (v0 : value) (T : ty),
-          (x |-> U; Gamma) |- v \Vin T -> empty |- v0 \Vin U -> Gamma |- [x := v0 ]v v \Vin T) ->
-      forall (Gamma : partial_map ty) (x : string) (U : ty) (v0 : value) (T : ty),
-        (x |-> U; Gamma) |- tvalue v \in T -> empty |- v0 \Vin U -> Gamma |- [x := v0] tvalue v \in T).
-Proof.
-  intros. inversion H0; clear H0; subst; simpl; eauto.
-Qed.
-
 Lemma substitution_preserves_typing7:
   (forall (s : string) (t : tm),
       (forall (Gamma : partial_map ty) (x : string) (U : ty) (v : value) (T : ty),
-          (x |-> U; Gamma) |- t \in T -> empty |- v \Vin U -> Gamma |- [x := v] t \in T) ->
+          (x |-> U; Gamma) |- t \Tin T -> empty |- v \Vin U -> Gamma |- [x := v] t \Tin T) ->
       forall t0 : tm,
         (forall (Gamma : partial_map ty) (x : string) (U : ty) (v : value) (T : ty),
-            (x |-> U; Gamma) |- t0 \in T -> empty |- v \Vin U -> Gamma |- [x := v] t0 \in T) ->
+            (x |-> U; Gamma) |- t0 \Tin T -> empty |- v \Vin U -> Gamma |- [x := v] t0 \Tin T) ->
         forall (Gamma : partial_map ty) (x : string) (U : ty) (v : value) (T : ty),
-          (x |-> U; Gamma) |- tlete s t t0 \in T -> empty |- v \Vin U -> Gamma |- [x := v] tlete s t t0 \in T).
+          (x |-> U; Gamma) |- tlete s t t0 \Tin T -> empty |- v \Vin U -> Gamma |- [x := v] tlete s t t0 \Tin T).
 Proof.
   intros. inversion H1; clear H1; subst; simpl; eauto.
   rename s into y. rename x into x.
@@ -194,31 +235,6 @@ Proof.
     rewrite update_permute in H9; auto. apply H0 with (U:=U); auto.
 Qed.
 
-Lemma substitution_preserves_typing8:
-  (forall (s : string) (b : biop) (v : value),
-      (forall (Gamma : partial_map ty) (x : string) (U : ty) (v0 : value) (T : ty),
-          (x |-> U; Gamma) |- v \Vin T -> empty |- v0 \Vin U -> Gamma |- [x := v0 ]v v \Vin T) ->
-      forall v0 : value,
-        (forall (Gamma : partial_map ty) (x : string) (U : ty) (v1 : value) (T : ty),
-            (x |-> U; Gamma) |- v0 \Vin T -> empty |- v1 \Vin U -> Gamma |- [x := v1 ]v v0 \Vin T) ->
-        forall t : tm,
-          (forall (Gamma : partial_map ty) (x : string) (U : ty) (v1 : value) (T : ty),
-              (x |-> U; Gamma) |- t \in T -> empty |- v1 \Vin U -> Gamma |- [x := v1] t \in T) ->
-          forall (Gamma : partial_map ty) (x : string) (U : ty) (v1 : value) (T : ty),
-            (x |-> U; Gamma) |- tletbiop s b v v0 t \in T ->  empty |- v1 \Vin U -> Gamma |- [x := v1] tletbiop s b v v0 t \in T).
-Proof.
-  intros. inversion H2; clear H2; subst; simpl; eauto.
-  rename s into y. rename x into x.
-  destruct (eqb_spec x y); subst.
-  + (* x=y *)
-    rewrite update_shadow in H13.
-    apply T_LetOp; auto. apply H with (U:=U); auto. apply H0 with (U:=U); auto.
-  + (* x<>y *)
-    apply T_LetOp; auto. apply H with (U:=U); auto.
-    rewrite update_permute in H13; auto. apply H0 with (U:=U); auto.
-    rewrite update_permute in H13; auto. apply H1 with (U:=U); auto.
-Qed.
-
 Lemma substitution_preserves_typing9:
   (forall (s : string) (v : value),
       (forall (Gamma : partial_map ty) (x : string) (U : ty) (v0 : value) (T : ty),
@@ -228,9 +244,9 @@ Lemma substitution_preserves_typing9:
             (x |-> U; Gamma) |- v0 \Vin T -> empty |- v1 \Vin U -> Gamma |- [x := v1 ]v v0 \Vin T) ->
         forall t : tm,
           (forall (Gamma : partial_map ty) (x : string) (U : ty) (v1 : value) (T : ty),
-              (x |-> U; Gamma) |- t \in T -> empty |- v1 \Vin U -> Gamma |- [x := v1] t \in T) ->
+              (x |-> U; Gamma) |- t \Tin T -> empty |- v1 \Vin U -> Gamma |- [x := v1] t \Tin T) ->
           forall (Gamma : partial_map ty) (x : string) (U : ty) (v1 : value) (T : ty),
-            (x |-> U; Gamma) |- tletapp s v v0 t \in T -> empty |- v1 \Vin U -> Gamma |- [x := v1] tletapp s v v0 t \in T).
+            (x |-> U; Gamma) |- tletapp s v v0 t \Tin T -> empty |- v1 \Vin U -> Gamma |- [x := v1] tletapp s v v0 t \Tin T).
 Proof.
   intros. inversion H2; clear H2; subst; simpl; eauto.
   rename s into y. rename x into x.
@@ -247,14 +263,15 @@ Proof.
 Qed.
 
 Lemma substitution_preserves_typing : forall t Gamma x U v T,
-    (x |-> U ; Gamma) |- t \in T ->  empty |- v \Vin U  ->  Gamma |- [x:=v]t \in T.
+    (x |-> U ; Gamma) |- t \Tin T ->  empty |- v \Vin U  ->  Gamma |- [x:=v]t \Tin T.
 Proof with eauto.
   intro t.
   apply (tm_mutual_rec
            (fun ev => forall Gamma x U v T, (x |-> U ; Gamma) |- ev \Vin T ->  empty |- v \Vin U ->  Gamma |- [x:=v]v ev \Vin T)
-           (fun e => forall Gamma x U v T, (x |-> U ; Gamma) |- e \in T ->  empty |- v \Vin U ->  Gamma |- [x:=v] e \in T)).
+           (fun e => forall Gamma x U v T, (x |-> U ; Gamma) |- e \Tin T ->  empty |- v \Vin U ->  Gamma |- [x:=v] e \Tin T)).
+  - intro c. induction c; intros; inversion H; clear H; subst; simpl; eauto; constructor...
   - intro c. destruct c.
-    + induction c; intros; inversion H; clear H; subst; simpl; eauto.
+    + intros. inversion H; clear H; subst; simpl; eauto; constructor...
     + apply substitution_preserves_typing2.
   - intros. inversion H0; subst; simpl; eauto.
     destruct (eqb_spec x s); subst.
@@ -263,14 +280,20 @@ Proof with eauto.
   - intros. inversion H0; subst; simpl; eauto.
   - intros. inversion H0; subst; simpl; eauto.
   - apply substitution_preserves_typing7.
-  - apply substitution_preserves_typing8.
+  - intros x op v1 Hv1 v2 Hv2 e He Gamma y U v_y T HTop HTs.
+    inversion HTop; subst. inversion H8; subst. simpl.
+    destruct (eqb_spec y x); subst; eapply T_LetOp...
+    + erewrite <- update_shadow...
+    + eapply He... erewrite update_permute...
   - apply substitution_preserves_typing9.
+  - intros v Hv e1 He1 e2 He2 Gamma y U v_y T HTmatch HTy. inversion HTmatch; subst.
+    simpl. eapply T_Matchb...
 Qed.
 
 Theorem preservation : forall t t' T,
-    empty |- t \in T  ->
+    empty |- t \Tin T  ->
                   t --> t'  ->
-                  empty |- t' \in T.
+                  empty |- t' \Tin T.
 Proof with eauto.
   intros t t' T HT. generalize dependent t'.
   remember empty as Gamma.
@@ -278,20 +301,19 @@ Proof with eauto.
     intros t' HE; subst; inversion HE; subst...
   - apply substitution_preserves_typing with T1...
     inversion HT1; subst...
-  - apply substitution_preserves_typing with (TBasic (op_ret_ty op))...
-  (* - apply substitution_preserves_typing with TNat... *)
+  - eapply substitution_preserves_typing...
   - apply T_Lete with (T1 := T_y)...
     apply substitution_preserves_typing with T_x...
     inversion H0; subst...
 Qed.
 
 Theorem preservation_value : forall t (v: value) T,
-    empty |- t \in T  -> t -->* v  ->
+    empty |- t \Tin T  -> t -->* v  ->
                   empty |- v \Vin T.
 Proof.
 Admitted.
 
-Definition any_ctx_const_nat_typed_is_nat: forall Gamma (c: constant), Gamma |- c \Vin TNat -> exists (n: nat), c = n.
-Proof with eauto.
-  intros. inversion H; subst. exists n...
-Qed.
+(* Definition any_ctx_const_nat_typed_is_nat: forall Gamma (c: constant), Gamma |- c \Vin TNat -> exists (n: nat), c = n. *)
+(* Proof with eauto. *)
+(*   intros. inversion H; subst. exists n... *)
+(* Qed. *)
