proof/RfTypeDef.v
@@ -3,56 +3,67 @@ From PLF Require Import Maps.
 From PLF Require Import Types.
 (* From PLF Require Import Smallstep. *)
 From PLF Require Import CoreLangSimp.
+From Coq Require Import Logic.FunctionalExtensionality.
+From Coq Require Import Logic.ClassicalFacts.
 
 Definition state := total_map constant.
 (* The second constant is the self reference; the refinement is untyped *)
 Definition refinement : Type := state -> constant -> Prop.
 Implicit Type HH : refinement.
 
-Definition refinment_subst (x:string) (c:constant) (phi:refinement) : refinement :=
-  fun st v => phi (t_update st x c) v.
-
 Inductive overbasety : Type :=
-| BaseOver: basic_ty -> refinement -> overbasety.
+| BaseOver: base_ty -> refinement -> overbasety.
 
-Definition overbasety_subst (x:string) (c:constant) (oty:overbasety) : overbasety :=
-  match oty with
-  | BaseOver T phi => BaseOver T (refinment_subst x c phi)
-  end.
+Global Hint Constructors overbasety: core.
 
-Inductive underarrowty : Type :=
-| DependArrow : string -> overbasety -> underty -> underarrowty
-| IndependArrow : underarrowty -> underty -> underarrowty
-with underty: Type :=
-| BaseUnder: basic_ty -> refinement -> underty
-| ArrowUnder: underarrowty -> underty.
+Inductive underty : Type :=
+| BaseUnder: base_ty -> refinement -> underty
+| DependArrow : string -> overbasety -> underty -> underty
+| IndependArrow : underty -> underty -> underty.
 
-Scheme underarrowty_mutual_rec := Induction for underarrowty Sort Type
-    with underty_mutual_rec := Induction for underty Sort Type.
+Global Hint Constructors underty: core.
 
-Fixpoint underarrowty_subst (id:string) (c:constant) (oty:underarrowty) : underarrowty :=
-  match oty with
-  | DependArrow x t1 t2 => DependArrow x (overbasety_subst id c t1)
-                                      (if String.eqb x id then t2 else underty_subst id c t2)
-  | IndependArrow t1 t2 => IndependArrow (underarrowty_subst id c t1) (underty_subst id c t2)
-  end
-with underty_subst (id:string) (c:constant) (oty:underty) : underty :=
-       match oty with
-       | BaseUnder T phi => BaseUnder T (refinment_subst id c phi)
-       | ArrowUnder ty => ArrowUnder (underarrowty_subst id c ty)
-       end.
+(* Fixpoint well_formed_underty_bool (tau: underty): bool := *)
+(*   match tau with *)
+(*   | BaseUnder _ _ => true *)
+(*   | DependArrow _ _ tau => well_formed_underty_bool tau *)
+(*   | IndependArrow t1 t2 => *)
+(*       if well_formed_underty_bool t2 *)
+(*       then *)
+(*         match t1 with *)
+(*         | BaseUnder _ _ => false *)
+(*         | _ => well_formed_underty_bool t1 *)
+(*         end *)
+(*       else *)
+(*         false *)
+(*   end. *)
+
+Inductive well_formed_underty: underty -> Prop :=
+| well_formed_underty_base: forall T phi, well_formed_underty (BaseUnder T phi)
+| well_formed_underty_oarr: forall a T phi tau, well_formed_underty tau -> well_formed_underty (DependArrow a (BaseOver T phi) tau)
+| well_formed_underty_arrarr1: forall a tau_a tau tau',
+    well_formed_underty (DependArrow a tau_a tau) -> well_formed_underty tau' ->
+    well_formed_underty (IndependArrow (DependArrow a tau_a tau) tau')
+| well_formed_underty_arrarr2: forall t1 t2 tau',
+    well_formed_underty (IndependArrow t1 t2) -> well_formed_underty tau' ->
+    well_formed_underty (IndependArrow (IndependArrow t1 t2) t2).
+
+Global Hint Constructors well_formed_underty: core.
+
+(* Definition well_formed_underty (tau : underty): Prop := well_formed_underty_bool tau = true. *)
 
 Inductive overunderty : Type :=
 | Uty: underty -> overunderty
 | Oty: overbasety -> overunderty.
 
-Definition overunderty_subst (id:string) (c:constant) (oty:overunderty) : overunderty :=
-  match oty with
-  | Uty ty => Uty (underty_subst id c ty)
-  | Oty ty => Oty (overbasety_subst id c ty)
-  end.
+Global Hint Constructors overunderty: core.
 
-Coercion ArrowUnder :underarrowty >-> underty.
+Inductive well_formed_type: overunderty -> Prop :=
+| well_formed_type_over: forall (tau: overbasety), well_formed_type (Oty tau)
+| well_formed_type_under: forall tau, well_formed_underty tau -> well_formed_type (Uty tau).
+
+Global Hint Constructors well_formed_type: core.
+
 Coercion Uty : underty >-> overunderty.
 Coercion Oty : overbasety >-> overunderty.
 
@@ -61,21 +72,17 @@ Definition over_to_under (ot: overbasety) :=
   | BaseOver t phi => BaseUnder t phi
   end.
 
-Notation "'[[v:' t '|' r ']]'" := (BaseUnder t r) (at level 20).
-Notation "'{{v:' t '|' r '}}'" := (BaseOver t r) (at level 20).
-Notation " x 'o:' overbasety 'o-->' retty " := (DependArrow x overbasety retty) (at level 20).
-Notation " underty 'u-->' retty " := (IndependArrow underty retty) (at level 20).
+Notation "'[[v:' t '|' r ']]'" := (BaseUnder t r) (at level 80).
+Notation "'{{v:' t '|' r '}}'" := (BaseOver t r) (at level 80).
+Notation " x 'o:' overbasety 'o-->' retty " := (DependArrow x overbasety retty) (at level 80).
+Notation " underty 'u-->' retty " := (IndependArrow underty retty) (at level 80).
 
-Fixpoint underarrowty_erase (ut: underarrowty) : ty :=
+Fixpoint underty_erase (ut: underty) : ty :=
   match ut with
+  | [[v: T | _ ]] => T
   | _ o: {{v: T1 | _ }} o--> retty => T1 t--> (underty_erase retty)
-  | t1 u--> t2 => (underarrowty_erase t1) t--> (underty_erase t2)
-  end
-with underty_erase (ut: underty) : ty :=
-       match ut with
-       | [[v: T | _ ]] => T
-       | ArrowUnder ut => underarrowty_erase ut
-       end.
+  | t1 u--> t2 => (underty_erase t1) t--> (underty_erase t2)
+  end.
 
 Definition overbasety_erase (aty: overbasety): ty :=
   match aty with
@@ -92,7 +99,6 @@ Notation " 'u\_' ty '_/' " := (underty_erase ty) (at level 30).
 Notation " 'o\_' ty '_/' " := (overbasety_erase ty) (at level 30).
 Notation " 'ou\_' ty '_/' " := (overunderty_erase ty) (at level 30).
 
-
 Definition eval_cid (st: state) (v: cid) :=
   match v with
   | vconst c => c
@@ -100,5 +106,135 @@ Definition eval_cid (st: state) (v: cid) :=
   end.
 
 Definition mk_op_retty_from_cids (op: biop) (cid1 cid2: cid): underty :=
-  BaseUnder (op_ret_ty op)
-  (fun st c => (exists (n1 n2: nat), eval_cid st cid1 = n1 /\ eval_cid st cid2 = n2 /\ c = apply_op op n1 n2)).
+  BaseUnder (ret_ty_of_op op) (fun st c => eval_op op (eval_cid st cid1) (eval_cid st cid2) c).
+
+(* closed_refinement *)
+
+Definition is_closed_refinement (_: base_ty) (phi: refinement): Prop := forall st st', phi st = phi st'.
+
+Global Hint Unfold is_closed_refinement: core.
+
+Lemma constant_refinement_is_closed: forall (c: constant) (phi: refinement),
+    (forall st : state, phi st = (fun c' => c = c')) -> (forall T, is_closed_refinement T phi).
+Proof.
+  intros.
+  intros st st'. rewrite H. rewrite H. auto.
+Qed.
+
+(* subst id *)
+Definition refinement_subst_id (x1 x2: string) (phi: refinement): refinement :=
+  (fun st c => phi (t_update st x1 (st x2)) c).
+
+Definition over_subst_id (x1 x2: string) (oty: overbasety): overbasety :=
+  match oty with
+  | BaseOver T phi => BaseOver T (refinement_subst_id x1 x2 phi)
+  end.
+
+Fixpoint under_subst_id (x1 x2: string) (uty: underty): underty :=
+  match uty with
+  | BaseUnder T phi => BaseUnder T (refinement_subst_id x1 x2 phi)
+  | DependArrow x xty retty =>
+      if String.eqb x1 x then
+        DependArrow x (over_subst_id x1 x2 xty) retty
+      else
+        DependArrow x (over_subst_id x1 x2 xty) (under_subst_id x1 x2 retty)
+  | IndependArrow t1 t2 =>
+      IndependArrow (under_subst_id x1 x2 t1) (under_subst_id x1 x2 t2)
+  end.
+
+Definition overunder_subst_id (x1: string) (c2: string) (outy: overunderty): overunderty :=
+  match outy with
+  | Uty uty => under_subst_id x1 c2 uty
+  | Oty oty => over_subst_id x1 c2 oty
+  end.
+
+Notation " '<r[' x '|id->' y ']>' uty " := (refinement_subst_id x y uty) (at level 40).
+Notation " '<u[' x '|id->' y ']>' uty " := (under_subst_id x y uty) (at level 40).
+Notation " '<o[' x '|id->' y ']>' uty " := (over_subst_id x y uty) (at level 40).
+Notation " '<ou[' x '|id->' y ']>' uty " := (overunder_subst_id x y uty) (at level 40).
+
+(* subst constant *)
+Definition refinement_subst_c (x1: string) (c2: constant) (phi: refinement): refinement :=
+  (fun st => phi (t_update st x1 c2)).
+
+Lemma refinement_subst_c_closed_rf: forall x1 c2 T phi,
+    is_closed_refinement T phi -> refinement_subst_c x1 c2 phi = phi.
+Proof.
+  intros.
+  unfold is_closed_refinement in H. unfold refinement_subst_c.
+  apply functional_extensionality. intros st.
+  erewrite H. reflexivity.
+Qed.
+
+Definition over_subst_c (x1: string) (c2: constant) (oty: overbasety): overbasety :=
+  match oty with
+  | BaseOver T phi => BaseOver T (refinement_subst_c x1 c2 phi)
+  end.
+
+Fixpoint under_subst_c (x1: string) (c2: constant) (uty: underty): underty :=
+  match uty with
+  | BaseUnder T phi => BaseUnder T (refinement_subst_c x1 c2 phi)
+  | DependArrow x xty retty =>
+      if String.eqb x1 x then
+        DependArrow x (over_subst_c x1 c2 xty) retty
+      else
+        DependArrow x (over_subst_c x1 c2 xty) (under_subst_c x1 c2 retty)
+  | IndependArrow t1 t2 =>
+      IndependArrow (under_subst_c x1 c2 t1) (under_subst_c x1 c2 t2)
+  end.
+
+Definition overunder_subst_c (x1: string) (c2: constant) (outy: overunderty): overunderty :=
+  match outy with
+  | Uty uty => under_subst_c x1 c2 uty
+  | Oty oty => over_subst_c x1 c2 oty
+  end.
+
+Notation " '<r[' x '|c->' y ']>' uty " := (refinement_subst_c x y uty) (at level 40).
+Notation " '<u[' x '|c->' y ']>' uty " := (under_subst_c x y uty) (at level 40).
+Notation " '<o[' x '|c->' y ']>' uty " := (over_subst_c x y uty) (at level 40).
+Notation " '<ou[' x '|c->' y ']>' uty " := (overunder_subst_c x y uty) (at level 40).
+
+Definition under_subst_cid (x1: string) (cv: cid) (outy: underty): underty :=
+  match cv with
+  | vconst c => under_subst_c x1 c outy
+  | vvar id => under_subst_id x1 id outy
+  end.
+
+(* appear free *)
+
+Definition appear_free_in_refinement (name: string) (phi: refinement): Prop :=
+  (exists st (c1 c2:constant),
+      phi (t_update st name c1) <> phi (t_update st name c2)
+  ).
+
+Definition appear_free_in_overbasety (name: string) (oty: overbasety): Prop :=
+  match oty with
+  | {{v: _ | phi }} => appear_free_in_refinement name phi
+  end.
+
+Fixpoint appear_free_in_underty (name: string) (uty: underty): Prop :=
+  match uty with
+  | [[v: _ | phi ]] => appear_free_in_refinement name phi
+  | DependArrow x xty retty =>
+      appear_free_in_overbasety name xty \/ (x <> name /\ appear_free_in_underty name retty)
+  | IndependArrow t1 t2 =>
+      appear_free_in_underty name t1 \/ appear_free_in_underty name t2
+  end.
+
+Definition appear_free_in_overunderty (name: string) (overunderty: overunderty): Prop :=
+  match overunderty with
+  | Uty uty => appear_free_in_underty name uty
+  | Oty oty => appear_free_in_overbasety name oty
+  end.
+
+Notation " x '\FVty' e " := (appear_free_in_overunderty x e) (at level 40).
+
+(* \S{Ty}: *)
+
+Definition mk_eq_constant c := [[v: ty_of_const c | (fun _ v => v = c) ]].
+Definition mk_bot ty := [[v: ty | (fun _ _ => False) ]].
+Definition mk_top ty := [[v: ty | (fun _ _ => True) ]].
+Definition mk_over_top ty := {{v: ty | (fun _ _ => True) }}.
+Definition mk_eq_var ty name := [[v: ty | (fun state v => v = (state name)) ]].
+Definition mk_op op a b :=
+  (a o: (mk_over_top (fst_ty_of_op op)) o--> (b o: (mk_over_top (fst_ty_of_op op)) o--> ([[v: ret_ty_of_op op | (fun st c => eval_op op (st a) (st b) c ) ]]))).
