proof/Soundness.v
@@ -4,7 +4,7 @@ From PLF Require Import CoreLangSimp.
 From PLF Require Import NormalTypeSystemSimp.
 From PLF Require Import LinearContext.
 From PLF Require Import RfTypeDef.
-From PLF Require Import WellFormedSimp.
+From PLF Require Import TypeClosedSimp.
 From PLF Require Import DenotationSimp.
 From PLF Require Import SubtypingSimp.
 From PLF Require Import TypingRules.
@@ -14,9 +14,9 @@ From Coq Require Import Lists.List.
 
 Import CoreLangSimp.
 Import LinearContext.
-Import WellFormedSimp.
+Import TypeClosedSimp.
 Import DenotationSimp.
-Import CtxInvariantSimp.
+Import WellFormedSimp.
 Import TypeDisj.
 Import SubtypingSimp.
 Import TypingRules.
@@ -26,21 +26,23 @@ Import ListNotations.
 (*     under_tmR ([[v:T | phi]]) e /\ (forall (c: constant), e -->* c <-> (forall st, phi st = (fun c' => c = c'))). *)
 (* Admitted. *)
 
-Lemma rf_nat_value_n_exists:
-  forall Gamma (v: cid) phi,
-    ctx_inv Gamma ->
-    Gamma \C- v \Vin ([[v:TNat | phi]]) ->
-    tmR_in_ctx Gamma ([[v:TNat | phi]]) v -> ((exists n, v = cnat n) \/ (exists x, v = vvar x)).
-Proof.
-  intros Gamma v phi Hinv H HD.
-  apply UT_Value in H. apply type_judgement_implies_basic_type_judgement in H. simpl in H.
-  destruct v.
-  - left. inversion H; subst. apply any_ctx_const_nat_typed_is_nat in H2. destruct H2 as (n & Hn). exists n... inversion Hn... reflexivity.
-  - right. exists s... reflexivity.
-Qed.
+(* Lemma rf_nat_value_n_exists: *)
+(*   forall Gamma (v: cid) phi, *)
+(*     ctx_inv Gamma -> *)
+(*     Gamma \C- v \Vin ([[v:TNat | phi]]) -> *)
+(*     tmR_in_ctx Gamma ([[v:TNat | phi]]) v -> ((exists n, v = cnat n) \/ (exists x, v = vvar x)). *)
+(* Proof. *)
+(*   intros Gamma v phi Hinv H HD. *)
+(*   apply UT_Value in H. apply type_judgement_implies_basic_type_judgement in H. simpl in H. *)
+(*   destruct v. *)
+(*   - left. inversion H; subst. apply any_ctx_const_nat_typed_is_nat in H2. destruct H2 as (n & Hn). exists n... inversion Hn... reflexivity. *)
+(*   - right. exists s... reflexivity. *)
+(* Qed. *)
 
 Global Hint Resolve ctx_inv_implies_fresh_binding_last: core.
-Global Hint Resolve ctx_inv_implies_well_found_last: core.
+Global Hint Resolve ctx_inv_implies_type_closed_last: core.
+
+Global Hint Rewrite app_nil_r: core.
 
 Theorem soundness: forall (Gamma: context) (e: tm) (uty:underty),
     Gamma \C- e \Tin uty -> tmR_in_ctx Gamma uty e.
@@ -50,69 +52,92 @@ Proof with eauto.
            (fun Gamma e uty H => tmR_in_ctx Gamma uty e)); intros Gamma.
   (* constant *)
   - intros c Hinv.
-    apply tmR_in_ctx_pre_weakening with (Gamma1 := Gamma) (Gamma2 := l_empty); auto. rewrite app_nil_r...
-  (* var under *)
-  - intros x tau Hinv Hfind. apply l_find_right_most_some_spec in Hfind.
-    destruct Hfind as (Gamma1 & Gamma2 & Hctxconcat & HGamma2). subst.
-    rewrite app_assoc... rewrite app_assoc in Hinv.
-    eapply tmR_in_ctx_post_weakening with (Gamma2 := Gamma2)...
-    + apply ctx_inv_implies_prefix_ctx_inv in Hinv...
-    + apply under_variable_has_same_type_in_ctx...
-   (* var over *)
+    apply tmR_in_ctx_pre_weakening with (Gamma1 := Gamma) (Gamma2 := l_empty); auto. rewrite app_nil_r... constructor...
+  (* op *)
+  - intros op a b (Hinv & Hclosed) Hab. apply tmR_in_ctx_pre_weakening with (Gamma1 := Gamma) (Gamma2 := l_empty); auto.
+    rewrite app_nil_r... constructor...
+  (* var over base *)
   - intros T x Hinv (phi & Hfind). apply l_find_right_most_some_spec in Hfind.
     destruct Hfind as (Gamma1 & Gamma2 & Hctxconcat & HGamma2). subst.
-    rewrite app_assoc. rewrite app_assoc in Hinv.
+    rewrite app_assoc. rewrite app_assoc in Hinv. inversion Hinv; subst.
     eapply tmR_in_ctx_post_weakening with (Gamma1 := (Gamma1 ++ ((x, Oty ({{v:T | phi}}))::nil))) (Gamma2 := Gamma2)...
     apply over_variable_has_eq_type_in_ctx.
+  (* var under base *)
+  - intros T x (Hinv & Hclosed) (phi & Hfind). apply l_find_right_most_some_spec in Hfind.
+    destruct Hfind as (Gamma1 & Gamma2 & Hctxconcat & HGamma2). subst.
+    rewrite app_assoc. rewrite app_assoc in Hinv.
+    eapply tmR_in_ctx_post_weakening with (Gamma1 := (Gamma1 ++ ((x, Uty ([[v:T | phi]]))::nil))) (Gamma2 := Gamma2)...
+    apply under_variable_has_eq_type_in_ctx...
+  (* var under arrarr *)
+  - intros x t1 t2 (Hinv & Hclosed) Hfind. apply l_find_right_most_some_spec in Hfind.
+    destruct Hfind as (Gamma1 & Gamma2 & Hctxconcat & HGamma2). subst.
+    eapply tmR_in_ctx_post_weakening with (Gamma1:= Gamma1 ++ ((x, Uty (t1 u--> t2))::nil)) (Gamma2 := Gamma2)... rewrite app_assoc...
+    + eapply ctx_inv_implies_mem_fresh_and_close...
+    + apply under_variable_has_same_type_in_ctx...
+  (* var under oarr *)
+  - intros x a tau_a tau_b (Hinv & Hclosed) Hfind. apply l_find_right_most_some_spec in Hfind.
+    destruct Hfind as (Gamma1 & Gamma2 & Hctxconcat & HGamma2). subst.
+    eapply tmR_in_ctx_post_weakening with (Gamma1:= Gamma1 ++ ((x, Uty (a o: tau_a o--> tau_b))::nil)) (Gamma2 := Gamma2)... rewrite app_assoc...
+    + eapply ctx_inv_implies_mem_fresh_and_close...
+    + apply under_variable_has_same_type_in_ctx...
   (* lam *)
-  - intros. apply tmR_in_ctx_preserve_oarr...
-  - intros. apply tmR_in_ctx_preserve_arrarr...
+  - intros x tau_x e tau (Hinv & Hclosed) He HeD.
+    assert (well_formed (Gamma <l> x :l: tau_x) tau) as HH. apply type_judgement_implies_inv in He...
+    destruct HH as (Hinv' & Hclosed'). apply tmR_in_ctx_preserve_oarr... inversion Hinv'; subst...
+  - intros x tau_x e tau Hwf He HeD.
+    assert (well_formed (Gamma <l> x :l: tau_x) tau) as HH. apply type_judgement_implies_inv in He...
+    destruct HH as (Hinv' & Hclosed').
+    apply tmR_in_ctx_preserve_arrarr... inversion Hinv'; subst...
   (* value *)
   - auto.
   (* err *)
-  - intros T Hinv.
+  - intros T (Hinv & Hclosed).
     assert (tmR_in_ctx l_empty (mk_bot T) texn)... unfold mk_bot.
     repeat constructor... intros. inversion H0.
     apply tmR_in_ctx_pre_weakening with (Gamma1 := Gamma) (Gamma2 := l_empty)... rewrite app_nil_r...
     constructor...
   (* sub *)
-  - intros e tau1 tau2 Ht1 Hd1 Hsub Hwf2 Hctx.
+  - intros e tau1 tau2 (Hinv & Hclosed) He HeD Hsub.
     apply is_subtype_spec with (e:=e) in Hsub...
-    eapply tmR_in_ctx_pre_weakening... apply app_nil_r.
+    eapply tmR_in_ctx_pre_weakening with (Gamma1 := Gamma) (Gamma2 := l_empty)... apply app_nil_r...
+    inversion Hsub; subst. eapply denotation_is_closed...
   (* eq *)
-  - intros e tau1 tau2 He HeD Hsub1 Hsub2 Hwf Hinv.
+  - intros e tau1 tau2 (Hinv & Hclosed) He HeD Hsub1 Hsub2.
     eapply is_subtype_spec...
   (* merge *)
-  - intros e tau1 tau2 tau3 He1 He1D He2 He2D Hdisj Hwf. unfold disjunct in Hdisj. rewrite <- Hdisj...
+  - intros e tau1 tau2 tau3 (Hinv & Hclosed) He1 He1D He2 He2D Hdisj. unfold disjunct in Hdisj. rewrite <- Hdisj...
   (* lete *)
-  - intros x e_x e tau tau_x Hex HexD He HeD Hwf.
+  - intros x e_x e tau tau_x (Hinv & Hclosed) Hex HexD He HeD.
     assert (ctx_inv (Gamma <l> x :l: tau_x)). eapply type_judgement_implies_inv...
     apply lete_ctx_inv_implies_safe_dropping_1_to_1 with (x:=x) (tau:=tau) (e:=e) (tau_x := tau_x)...
   (* letop *)
-  - intros x op v1 v2 e tau phi1 phi2 Hv1 Hv1D Hv2 Hv2D He HeD Hwf.
+  - intros x op v1 v2 e tau phi1 phi2 (Hinv & Hclosed) Hv1 Hv1D Hv2 Hv2D He HeD.
     assert (ctx_inv (Gamma <l> x :l: (mk_op_retty_from_cids op v1 v2))). eapply type_judgement_implies_inv...
     assert (ctx_inv Gamma). eapply type_judgement_implies_inv... constructor...
     apply tletbiop_ctx_inv_implies_safe_dropping_1_to_1...
   (* letapp_arrarr *)
-  - intros x v1 v2 e tau tauarg tau_x Hv1 Hv1D Hv2 Hv2D He HeD Hwf.
+  - intros x v1 v2 e tau tauarg tau_x (Hinv & Hclosed) Hv1 Hv1D Hv2 Hv2D He HeD.
     assert (ctx_inv (Gamma <l> x :l: tau_x)). eapply type_judgement_implies_inv...
     assert (ctx_inv Gamma). eapply type_judgement_implies_inv... constructor...
     eapply tletapp_arrarr_ctx_inv_implies_safe_dropping_1_to_1...
-  (* letapp_const *)
-  - intros x v1 c2 e tau T phi a tau_x Hv1 Hv1D Hv2 Hv2D He HeD Hwf.
+  (* letapp_oarr *)
+  - intros x v1 c2 e tau T phi a tau_x (Hinv & Hclosed) Hv1 Hv1D Hv2 Hv2D He HeD.
     assert (ctx_inv (Gamma <l> x :l: (under_subst_cid a c2 tau_x))). eapply type_judgement_implies_inv...
     assert (ctx_inv Gamma). eapply type_judgement_implies_inv... constructor...
     eapply tletapp_oarr_ctx_inv_implies_safe_dropping_1_to_1...
+  (* matchb true *)
+  - intros v e1 e2 tau (Hinv & Hclosed) Hv HvD He1 He1D. eapply tmR_in_ctx_preserve_matchb_true...
+  - intros v e1 e2 tau (Hinv & Hclosed) Hv HvD He1 He1D. eapply tmR_in_ctx_preserve_matchb_false...
 Qed.
 
-Lemma coverage: forall (e: tm) (T:basic_ty) (phi: constant -> Prop),
-    l_empty \C- e \Tin [[v: T | fun _ c => phi c ]] ->
+Lemma coverage: forall (e: tm) (T:base_ty) (phi: constant -> Prop),
+    l_empty \C- e \Tin ([[v: T | fun _ c => phi c ]]) ->
     forall (c: constant), empty |- (vconst c) \Vin T -> phi c -> e -->* vconst c .
 Proof with eauto.
   intros.
   apply soundness in H.
   inversion H; subst.
-  inversion H2; subst. simpl in H2, H4.
-  destruct H4 as (_ & _ & Hprop).
+  inversion H2; subst. simpl in H2, H5.
+  destruct H5 as (_ & _ & Hprop).
   apply Hprop; auto.
 Qed.
