proof/TermOrdering.v
@@ -1,0 +1,53 @@
+(** * MoreStlc: More on the Simply Typed Lambda-Calculus *)
+
+Set Warnings "-notation-overridden,-parsing".
+From PLF Require Import Maps.
+From PLF Require Import CoreLangSimp.
+From PLF Require Import NormalTypeSystemSimp.
+From Coq Require Import Logic.FunctionalExtensionality.
+From Coq Require Import Logic.ClassicalFacts.
+From Coq Require Import Lists.List.
+
+Import CoreLangSimp.
+Import NormalTypeSystemSimp.
+Import ListNotations.
+
+Definition term_order (e e': tm) := (forall v, e -->* v -> e' -->* v).
+
+Notation " e1 '<-<' e2 " := (term_order e1 e2) (at level 90).
+
+Notation " e1 '<=<' e2 " := (term_order e1 e2 /\ term_order e2 e1) (at level 90).
+
+Lemma term_order_trans (e1 e2 e3: tm): e1 <-< e2 -> e2 <-< e3 -> e1 <-< e3.
+Admitted.
+
+Global Hint Resolve term_order_trans: core.
+
+Lemma eta_reduction: forall x1 (f: value) x2 (v: value),
+    ~ x1 \FVvalue v ->
+    (tletapp x2 f v x2) <=< (tlete x1 f (tletapp x2 x1 v x2)).
+Admitted.
+
+Lemma eta_application_const_to_lete_const: forall x2 x T e (c_x: constant),
+    (tlete x c_x e) <=< (tletapp x2 (vlam x T e) c_x x2).
+Admitted.
+
+Lemma eta_lete_const_to_subst: forall x e (c_x: constant),
+    (subst x c_x e) <=< (tlete x c_x e).
+Admitted.
+
+Lemma eta_lete_const_to_subst_in_lam: forall a T x e (c_x: constant),
+    (vlam a T (subst x c_x e)) <=< (vlam a T (tlete x c_x e)).
+Admitted.
+
+Lemma eta_closed_term_can_captured_by_lam: forall a e_a Ta x T e,
+    empty |- e_a \Tin Ta -> a <> x ->
+                    (vlam x T (tlete a e_a e)) <=< (tlete a e_a (vlam x T e)).
+Admitted.
+
+Lemma eta_matchb_true: forall e1 e2, e1 <=< (tmatchb true e1 e2).
+Admitted.
+
+Lemma eta_matchb_false: forall e1 e2, e2 <=< (tmatchb false e1 e2).
+Admitted.
+
