proof/TypeClosedSimp.v
@@ -1,0 +1,271 @@
+Set Warnings "-notation-overridden,-parsing".
+From PLF Require Import Maps.
+From PLF Require Import CoreLangSimp.
+From Coq Require Import Lists.List.
+From Coq Require Import Strings.String.
+From Coq Require Import Logic.FunctionalExtensionality.
+From Coq Require Import Logic.ClassicalFacts.
+From PLF Require Import NormalTypeSystemSimp.
+From PLF Require Import RfTypeDef.
+From PLF Require Import LinearContext.
+Import ListNotations.
+
+Definition ncontxt := linear_context ty.
+Definition lcontxt := linear_context overunderty.
+
+Fixpoint ncontxt_to_basic_ctx_aux (Gamma: ncontxt) (ctx: partial_map ty) :=
+  match Gamma with
+  | nil => ctx
+  | (x, xty) :: Gamma => ncontxt_to_basic_ctx_aux Gamma (update ctx x xty)
+  end.
+
+Definition ncontxt_to_basic_ctx (Gamma: ncontxt) := ncontxt_to_basic_ctx_aux Gamma empty.
+
+Global Hint Unfold ncontxt_to_basic_ctx: core.
+
+Inductive type_closed_refinement : ncontxt -> base_ty -> refinement -> Prop :=
+| type_closed_refinement_nil: forall T phi, is_closed_refinement T phi -> type_closed_refinement [] T phi
+| type_closed_refinement_cons: forall x T Gamma Tphi phi,
+    (forall (c_x: constant), empty |- c_x \Vin T ->
+                                type_closed_refinement Gamma Tphi (fun st c => phi (t_update st x c_x) c)) ->
+    type_closed_refinement ((x, T) :: Gamma) Tphi phi.
+
+Global Hint Constructors type_closed_refinement: core.
+
+Lemma type_closed_refinement_weakening: forall Gamma1 Gamma2 Gamma3 T phi,
+    (Gamma1 ++ Gamma2) = Gamma3 ->
+    type_closed_refinement Gamma2 T phi ->
+    type_closed_refinement Gamma3 T phi.
+Admitted.
+
+Module ExCloseRefinement.
+
+  Example true_refinement: is_closed_refinement TNat (fun _ c => c = 3).
+  Proof.
+    unfold is_closed_refinement. reflexivity.
+  Qed.
+
+  (* When the type dismatch, it is equal to bottom refinement *)
+  Example true_refinement2: is_closed_refinement TNat (fun _ c => c = true).
+  Proof.
+    unfold is_closed_refinement. reflexivity.
+  Qed.
+
+  Example refinement_under_nctx: type_closed_refinement [("x"%string, TBase TNat)] TNat (fun st c => c = st "x"%string).
+  Proof.
+    constructor. intros.
+    apply nat_value_n_exists in H. destruct H; subst.
+    constructor. constructor; subst; auto.
+  Qed.
+
+End ExCloseRefinement.
+
+Inductive overunderbasety : Type :=
+| Obase: base_ty -> refinement -> overunderbasety
+| Ubase: base_ty -> refinement -> overunderbasety.
+
+Definition basecontxt := linear_context overunderbasety.
+
+Fixpoint erase_basetypectx (Gamma: basecontxt): ncontxt :=
+  match Gamma with
+  | nil => nil
+  | (x, Obase T _)::Gamma => (x, TBase T)::(erase_basetypectx Gamma)
+  | (x, Ubase T _)::Gamma => (x, TBase T)::(erase_basetypectx Gamma)
+  end.
+
+Fixpoint erase_lctx (Gamma: lcontxt): ncontxt :=
+  match Gamma with
+  | nil => nil
+  | (x, tau)::Gamma => (x, ou\_ tau _/)::(erase_lctx Gamma)
+  end.
+
+Definition lctx_to_basic_ctx (Gamma: lcontxt) := ncontxt_to_basic_ctx_aux (erase_lctx Gamma) empty.
+
+Global Hint Unfold lctx_to_basic_ctx: core.
+
+Inductive type_closed_in_basectx : basecontxt -> overunderty -> Prop :=
+| type_closed_base1: forall Gamma (T: base_ty) phi,
+    type_closed_refinement (erase_basetypectx Gamma) T phi ->
+    type_closed_in_basectx Gamma ({{v: T | phi}})
+| type_closed_base2: forall Gamma (T: base_ty) phi,
+    type_closed_refinement (erase_basetypectx Gamma) T phi ->
+    type_closed_in_basectx Gamma ([[v: T | phi]])
+| type_closed_oarr: forall Gamma x T phi (tau: underty),
+    type_closed_in_basectx Gamma ({{v: T | phi}}) ->
+    type_closed_in_basectx ((x, Obase T phi) :: Gamma) tau ->
+    type_closed_in_basectx Gamma (x o: ({{v: T | phi}}) o--> tau)
+| type_closed_arrarr: forall Gamma (tau_x: underty) (tau: underty),
+    type_closed_in_basectx Gamma tau_x ->
+    type_closed_in_basectx Gamma tau ->
+    type_closed_in_basectx Gamma (tau_x u--> tau).
+
+Global Hint Constructors type_closed_in_basectx: core.
+
+(* before erase refinement from the context, we will erase all function type bindings *)
+Fixpoint lcontxt_to_baseconctx (Gamma: lcontxt): basecontxt :=
+  match Gamma with
+  | nil => nil
+  | (x, ty)::Gamma =>
+      match ty with
+      | Oty ({{v: T | phi }}) => (x, Obase T phi)::(lcontxt_to_baseconctx Gamma)
+      | Uty ([[v: T | phi ]]) => (x, Ubase T phi)::(lcontxt_to_baseconctx Gamma)
+      | _ => (lcontxt_to_baseconctx Gamma)
+      end
+  end.
+
+Definition type_closed (Gamma: lcontxt) (tau: overunderty):=
+  type_closed_in_basectx (lcontxt_to_baseconctx Gamma) tau.
+
+Global Hint Unfold type_closed: core.
+
+(* type closed \S{Ty} *)
+
+Lemma mk_op_is_type_closed: forall op a b, type_closed l_empty (mk_op op a b).
+Admitted.
+
+Global Hint Resolve mk_op_is_type_closed: core.
+
+Lemma mk_eq_over_base_is_type_closed: forall x T phi, type_closed ((x, Oty ({{v:T | phi}}))::nil) (mk_eq_var T x).
+Proof with eauto.
+  intros x T phi. repeat constructor...
+  unfold is_closed_refinement... intros st st'. rewrite t_update_eq. rewrite t_update_eq. reflexivity.
+Qed.
+
+Global Hint Resolve mk_eq_over_base_is_type_closed: core.
+
+Lemma mk_eq_under_base_is_type_closed: forall x T phi, type_closed ((x, Uty ([[v:T | phi]]))::nil) (mk_eq_var T x).
+Proof with eauto.
+  intros x T phi. repeat constructor...
+  unfold is_closed_refinement... intros st st'. rewrite t_update_eq. rewrite t_update_eq. reflexivity.
+Qed.
+
+Global Hint Resolve mk_eq_under_base_is_type_closed: core.
+
+Lemma mk_eq_constant_spec (c: constant) : empty |- vconst c \Tin u\_ mk_eq_constant c _/.
+Proof with eauto.
+  induction c; simpl; repeat constructor...
+Qed.
+
+Lemma subst_constant_eq: forall x c_x c, (<u[ x |c-> c_x ]> mk_eq_constant c) = mk_eq_constant c.
+Proof.
+  intros. simpl.
+  assert (<r[ x |c-> c_x ]> (fun (_ : state) (v : constant) => v = c) = (fun (_ : state) (v : constant) => v = c)).
+  unfold refinement_subst_c.
+  apply functional_extensionality. intros. apply functional_extensionality. auto.
+  setoid_rewrite H. auto.
+Qed.
+
+Lemma constant_eq_is_close: forall Gamma c, type_closed Gamma (mk_eq_constant c).
+Proof.
+  intros. constructor.
+  assert (type_closed_refinement nil (ty_of_const c) (fun (_ : state) (v : constant) => v = c)).
+  constructor.
+  unfold is_closed_refinement; destruct c; simpl; reflexivity.
+  apply type_closed_refinement_weakening with (Gamma1 := (erase_basetypectx (lcontxt_to_baseconctx Gamma))) (Gamma2 := nil); auto.
+  rewrite app_nil_r. auto.
+Qed.
+
+Global Hint Resolve mk_eq_constant_spec: core.
+Global Hint Resolve subst_constant_eq: core.
+Global Hint Resolve constant_eq_is_close: core.
+
+(* type closed lemmas *)
+
+Lemma type_closed_add_post: forall (Gamma1 Gamma2: lcontxt) (tau: overunderty),
+    type_closed Gamma1 tau -> type_closed (Gamma1 ++ Gamma2) tau.
+Admitted.
+
+Lemma type_closed_add_pre: forall (Gamma1 Gamma2: lcontxt) (tau: overunderty),
+    type_closed Gamma2 tau -> type_closed (Gamma1 ++ Gamma2) tau.
+Admitted.
+
+Lemma type_closed_drop_post: forall (Gamma1 Gamma2: lcontxt) (tau: overunderty),
+	(forall x tau_x, l_find_right_most Gamma2 x = Some tau_x -> ~ appear_free_in_overunderty x tau) ->
+	type_closed (Gamma1 ++ Gamma2) tau -> type_closed Gamma1 tau.
+Admitted.
+
+Global Hint Resolve type_closed_add_pre: core.
+Global Hint Resolve type_closed_add_post: core.
+
+Fixpoint erase_arr_bindings (Gamma: lcontxt): lcontxt :=
+  match Gamma with
+  | nil => nil
+  | (x, ty)::Gamma =>
+      match ty with
+      | Oty _ | Uty ([[v: _ | _ ]]) => (x, ty)::(erase_arr_bindings Gamma)
+      | _ => (erase_arr_bindings Gamma)
+      end
+  end.
+
+Lemma erase_arr_bindings_spec: forall (Gamma: lcontxt),
+    lcontxt_to_baseconctx Gamma = lcontxt_to_baseconctx (erase_arr_bindings Gamma).
+Proof.
+  intro Gamma. induction Gamma; auto.
+  destruct a as (x, xty).
+  destruct xty. destruct u; simpl; auto.
+  - rewrite IHGamma. auto.
+  - destruct o. simpl. rewrite IHGamma. auto.
+Qed.
+
+Lemma type_closed_even_without_arr_bindings: forall Gamma tau,
+    type_closed Gamma tau <-> type_closed (erase_arr_bindings Gamma) tau.
+Proof.
+  unfold type_closed. setoid_rewrite <- erase_arr_bindings_spec. reflexivity.
+Qed.
+
+Definition lcontxt_to_basic_ctx (Gamma: lcontxt) := ncontxt_to_basic_ctx (erase_basetypectx (lcontxt_to_baseconctx Gamma)).
+
+Global Hint Unfold lcontxt_to_basic_ctx: core.
+
+Inductive type_ctx_no_dup: lcontxt -> Prop :=
+| type_ctx_no_dup_nil: type_ctx_no_dup nil
+| type_ctx_no_dup_cons: forall x tau_x Gamma,
+    l_find_right_most Gamma x = None ->
+    type_ctx_no_dup (Gamma <l> x :l: tau_x).
+
+Global Hint Constructors type_ctx_no_dup: core.
+
+Lemma type_ctx_no_dup_fst_last_diff_name: forall a tau_a Gamma b tau_b,
+    type_ctx_no_dup ((a, tau_a)::Gamma ++ ((b, tau_b)::nil)) -> a <> b.
+Admitted.
+
+Global Hint Resolve type_ctx_no_dup_fst_last_diff_name: core.
+
+Lemma type_ctx_no_dup_ctx_sub: forall Gamma1 Gamma2,
+    type_ctx_no_dup (Gamma1 ++ Gamma2) -> type_ctx_no_dup Gamma1 /\ type_ctx_no_dup Gamma2.
+Admitted.
+
+Global Hint Resolve type_ctx_no_dup_ctx_sub: core.
+
+(* type_closed_ctx: *)
+(*   1. should also have no duplicate names *)
+(*   2. types are well_formed *)
+(*   3. types are closed *)
+
+Inductive type_closed_ctx: lcontxt -> Prop :=
+| type_closed_ctx_nil: type_closed_ctx nil
+| type_closed_ctx_cons: forall x tau_x Gamma,
+    l_find_right_most Gamma x = None ->
+    type_closed_ctx Gamma ->
+    type_closed Gamma tau_x ->
+    well_formed_type tau_x ->
+    type_closed_ctx (Gamma <l> x :l: tau_x).
+
+Global Hint Constructors type_closed_ctx: core.
+
+Lemma type_closed_ctx_implies_type_ctx_no_dup: forall Gamma, type_closed_ctx Gamma -> type_ctx_no_dup Gamma.
+Admitted.
+
+Global Hint Resolve type_closed_ctx_implies_type_ctx_no_dup: core.
+
+Lemma type_closed_ctx_fst_last_diff_name: forall a tau_a Gamma b tau_b,
+    type_closed_ctx ((a, tau_a)::Gamma ++ ((b, tau_b)::nil)) -> a <> b.
+Admitted.
+
+Lemma type_closed_ctx_prefix: forall Gamma1 Gamm2,
+    type_closed_ctx (Gamma1 ++ Gamm2) -> type_closed_ctx Gamma1.
+Admitted.
+
+Lemma type_closed_ctx_even_without_arr_bindings: forall Gamma,
+    type_closed_ctx Gamma -> type_closed_ctx (erase_arr_bindings Gamma).
+Admitted.
