proof/TypingRules.v
@@ -4,9 +4,9 @@ From PLF Require Import CoreLangSimp.
 From PLF Require Import NormalTypeSystemSimp.
 From PLF Require Import LinearContext.
 From PLF Require Import RfTypeDef.
-From PLF Require Import WellFormedSimp.
+From PLF Require Import TypeClosedSimp.
 From PLF Require Import DenotationSimp.
-From PLF Require Import CtxInvariantSimp.
+From PLF Require Import WellFormedSimp.
 From PLF Require Import TypeDisj.
 From PLF Require Import SubtypingSimp.
 From Coq Require Import Logic.FunctionalExtensionality.
@@ -15,9 +15,9 @@ From Coq Require Import Lists.List.
 
 Import CoreLangSimp.
 Import LinearContext.
-Import WellFormedSimp.
+Import TypeClosedSimp.
 Import DenotationSimp.
-Import CtxInvariantSimp.
+Import WellFormedSimp.
 Import TypeDisj.
 Import SubtypingSimp.
 Import ListNotations.
@@ -44,56 +44,74 @@ Reserved Notation "Gamma '\C-' t '\Vin' T" (at level 40).
 
 Inductive term_under_type_chek : context -> tm -> underty -> Prop :=
 | UT_Value: forall Gamma v uty, Gamma \C- v \Vin uty -> Gamma \C- (tvalue v) \Tin uty
-| UT_Exn: forall Gamma T, ctx_inv Gamma -> Gamma \C- texn \Tin (mk_bot T)
+| UT_Exn: forall Gamma T, well_formed Gamma (mk_bot T) -> Gamma \C- texn \Tin (mk_bot T)
 | UT_Sub: forall Gamma e tau1 tau2,
-    l_empty \C- e \Tin tau1 -> l_empty  \C- tau1 \<: tau2 ->
-    well_formed l_empty tau2 -> ctx_inv Gamma ->
+    well_formed Gamma tau2 ->
+    l_empty \C- e \Tin tau1 -> l_empty \C- tau1 \<: tau2 ->
     Gamma \C- e \Tin tau2
 | UT_Eq: forall Gamma e tau1 tau2,
+    well_formed Gamma tau2 ->
     Gamma \C- e \Tin tau1 ->
     Gamma \C- tau1 \<: tau2 -> Gamma \C- tau2 \<: tau1 ->
-    well_formed Gamma tau2 -> ctx_inv Gamma ->
     Gamma \C- e \Tin tau2
 | UT_Merge: forall Gamma e (tau1 tau2 tau3: underty),
+    well_formed Gamma tau3 ->
     Gamma \C- e \Tin tau1 -> Gamma \C- e \Tin tau2 -> (Gamma \C- tau1 \tyor tau2 \tyeq tau3) ->
-    well_formed l_empty tau3 ->
     Gamma \C- e \Tin tau3
 | UT_Lete: forall (Gamma: context) x e_x e tau, forall tau_x,
+    well_formed Gamma tau ->
     Gamma \C- e_x \Tin tau_x -> (Gamma <l> x :l: tau_x) \C- e \Tin tau ->
-    well_formed Gamma tau ->
     Gamma \C- (tlete x e_x e) \Tin tau
+(* operators only take nat type *)
 | UT_LetOp: forall (Gamma: context) x op (v1 v2: cid) e tau, forall phi1 phi2,
-    Gamma \C- v1 \Vin [[v: TNat | phi1 ]] ->
-    Gamma \C- v2 \Vin [[v: TNat | phi2 ]] ->
-    (Gamma <l> x :l: (mk_op_retty_from_cids op v1 v2)) \C- e \Tin tau ->
     well_formed Gamma tau ->
+    Gamma \C- v1 \Vin ([[v: TNat | phi1 ]]) ->
+    Gamma \C- v2 \Vin ([[v: TNat | phi2 ]]) ->
+    (Gamma <l> x :l: (mk_op_retty_from_cids op v1 v2)) \C- e \Tin tau ->
     Gamma \C- (tletbiop x op v1 v2 e) \Tin tau
 | UT_LetAppIndepend: forall Gamma x v1 v2 e tau, forall tauarg tau_x,
+    well_formed Gamma tau ->
     Gamma \C- v1 \Vin (tauarg u--> tau_x) -> Gamma \C- v2 \Vin tauarg ->
     (Gamma <l> x :l: tau_x) \C- e \Tin tau ->
-    well_formed Gamma tau ->
     Gamma \C- (tletapp x v1 v2 e) \Tin tau
 (* the value can only be constant or variables *)
-| UT_LetAppDepend1: forall Gamma x v1 (c2: cid) e tau, forall T phi a tau_x,
-    Gamma \C- v1 \Vin (a o: {{v: T | phi}} o--> tau_x) -> Gamma \C- c2 \Vin [[v: T | phi]] ->
-   (Gamma <l> x :l:(under_subst_cid a c2 tau_x)) \C- e \Tin tau ->
+| UT_LetAppDepend: forall Gamma x v1 (c2: cid) e tau, forall T phi a tau_x,
     well_formed Gamma tau ->
+    Gamma \C- v1 \Vin (a o: {{v: T | phi}} o--> tau_x) -> Gamma \C- c2 \Vin ([[v: T | phi]]) ->
+    (Gamma <l> x :l:(under_subst_cid a c2 tau_x)) \C- e \Tin tau ->
     Gamma \C- (tletapp x v1 c2 e) \Tin tau
+| UT_Matchb_true: forall Gamma v e1 e2 tau,
+    well_formed Gamma tau ->
+    Gamma \C- v \Vin (mk_eq_constant true) -> Gamma \C- e1 \Tin tau ->
+    Gamma \C- (tmatchb v e1 e2) \Tin tau
+| UT_Matchb_false: forall Gamma v e1 e2 tau,
+    well_formed Gamma tau ->
+    Gamma \C- v \Vin (mk_eq_constant false) -> Gamma \C- e2 \Tin tau ->
+    Gamma \C- (tmatchb v e1 e2) \Tin tau
 with value_under_type_check : context -> value -> underty -> Prop :=
-| UT_Contant: forall Gamma c, ctx_inv Gamma -> Gamma \C- (vconst c) \Vin (mk_eq_constant c)
-| UT_VarUnder: forall Gamma x (tau: underty),
-    ctx_inv Gamma -> l_find_right_most Gamma x = Some (Uty tau) ->  Gamma \C- (vvar x) \Vin tau
+| UT_Contant: forall Gamma (c: constant),
+    well_formed Gamma (mk_eq_constant c) -> Gamma \C- (vconst c) \Vin (mk_eq_constant c)
+| UT_Op: forall Gamma (op: biop) a b,
+    well_formed Gamma (mk_op op a b) -> a <> b -> Gamma \C- (vbiop op) \Vin (mk_op op a b)
 | UT_VarOver: forall Gamma T x,
-    ctx_inv Gamma -> (exists phi, l_find_right_most Gamma x = Some (Oty ({{v: T | phi}}))) ->
+    well_formed Gamma (mk_eq_var T x) -> (exists phi, l_find_right_most Gamma x = Some (Oty ({{v: T | phi}}))) ->
     Gamma \C- (vvar x) \Vin (mk_eq_var T x)
+| UT_VarUnderBase: forall Gamma T x,
+    well_formed Gamma (mk_eq_var T x) -> (exists phi, l_find_right_most Gamma x = Some (Uty ([[v: T | phi]]))) ->
+    Gamma \C- (vvar x) \Vin (mk_eq_var T x)
+| UT_VarUnderArrArr: forall Gamma x (t1 t2: underty),
+    well_formed Gamma (t1 u--> t2) -> l_find_right_most Gamma x = Some (Uty (t1 u--> t2)) -> Gamma \C- (vvar x) \Vin (t1 u--> t2)
+| UT_VarUnderOArr: forall Gamma x a tau_a (tau_b: underty),
+    well_formed Gamma (a o: tau_a o--> tau_b) -> l_find_right_most Gamma x = Some (Uty (a o: tau_a o--> tau_b)) ->
+    Gamma \C- (vvar x) \Vin (a o: tau_a o--> tau_b)
 | UT_LamDep: forall Gamma x tau_x e tau,
     well_formed Gamma (x o: tau_x o--> tau) ->
     (Gamma <l> x :l: Oty tau_x) \C- e \Tin tau ->
-                                          Gamma \C- (vlam x (o\_ tau_x _/) e) \Vin (x o: tau_x o--> tau)
+    Gamma \C- (vlam x (o\_ tau_x _/) e) \Vin (x o: tau_x o--> tau)
 | UT_LamIndep: forall Gamma x tau_x e tau,
     well_formed Gamma (tau_x u--> tau) ->
     (Gamma <l> x :l: Uty tau_x) \C- e \Tin tau ->
-                                          Gamma \C- (vlam x (u\_ tau_x _/) e) \Vin (tau_x u--> tau)
+    Gamma \C- (vlam x (u\_ tau_x _/) e) \Vin (tau_x u--> tau)
 where
 "Gamma '\C-' t '\Tin' T" := (term_under_type_chek Gamma t T) and "Gamma '\C-' t '\Vin' T" := (value_under_type_check Gamma t T).
 
@@ -108,9 +126,15 @@ Scheme value_under_type_check_rec := Induction for value_under_type_check Sort P
 (* Admitted. *)
 
 Lemma type_judgement_implies_inv: forall Gamma e tau,
-    Gamma \C- e \Tin tau -> ctx_inv Gamma /\ well_formed Gamma tau.
-Admitted.
+    Gamma \C- e \Tin tau -> well_formed Gamma tau.
+Proof.
+  intros.
+  induction H; auto.
+  - inversion H; auto.
+Qed.
+
+Global Hint Resolve type_judgement_implies_inv: core.
 
 Lemma type_judgement_implies_basic_type_judgement: forall Gamma e tau,
-    Gamma \C- e \Tin tau -> (lctx_to_basic_ctx Gamma) |- e \in u\_ tau _/.
+    Gamma \C- e \Tin tau -> (lctx_to_basic_ctx Gamma) |- e \Tin u\_ tau _/.
 Admitted.
